wip for refactoring

src/Utility.v
@@ -95,6 +95,8 @@ Class MachineWidth(t: Set) := mkMachineWidth {
   regToNat_natToReg_idemp: forall n : nat, n < pow2 XLEN -> regToNat (natToReg n) = n;
   *)
 
+  signed_eqb_spec: forall a b, signed_eqb a b = true <-> a = b;
+  
   regToZ_signed_bounds: forall a, - 2 ^ (XLEN - 1) <= regToZ_signed a < 2 ^ (XLEN - 1);
   regToZ_unsigned_bounds: forall a, 0 <= regToZ_unsigned a < 2 ^ XLEN;
 
@@ -122,6 +124,24 @@ Section DerivedProperties.
   Context {t: Set}.
   Context {MW: MachineWidth t}.
 
+  (* TODO rename signed_eqb to reg_eqb in Haskell *)
+  Definition reg_eqb := signed_eqb.
+
+  Definition XLEN_in_bytes: Z := XLEN / 8.
+
+  Lemma reg_eqb_true: forall a b, reg_eqb a b = true <-> a = b.
+  Proof.
+    unfold reg_eqb. exact signed_eqb_spec.
+  Qed.
+
+  Lemma reg_eqb_false: forall a b, reg_eqb a b = false <-> a <> b.
+  Proof.
+    intros. split; intros.
+    - intro. rewrite <- reg_eqb_true in H0. congruence.
+    - destruct (reg_eqb a b) eqn: E; try congruence.
+      exfalso. apply H. apply reg_eqb_true in E. assumption.
+  Qed.
+  
   Lemma add_def_unsigned: forall a b, add a b = ZToReg (regToZ_unsigned a + regToZ_unsigned b).
   Admitted.
   
